proofs/LibcruxAesgcm.lean
@@ -59,7 +59,7 @@ aes_core.transpose_u16x8.transpose_u16x8 input output
 
           simp only [<- var_3, <- var_6, <- var_8, <- var_11, <- var_13, <- var_16, <- var_18, <- var_44]
 
-          bv_check "./sat_proofs/LibcruxAesgcm.lean-aes_core.transpose_u16x8_correct-59-10.lrat"
+          bv_check "./sat_proofs/transpose_u16x8_correct.lrat"
     all_goals try omega
     grind
 
@@ -95,7 +95,7 @@ aes_core.transpose_u8x16.transpose_u8x16 input output
             <- var_17, <- var_20, <- var_22, <- var_25, <- var_27, <- var_30,
             <- var_32, <- var_35, <- var_37]
 
-          bv_check "./sat_proofs/LibcruxAesgcm.lean-aes_core.transpose_u8x16_correct-96-10.lrat"
+          bv_check "./sat_proofs/transpose_u8x16_correct.lrat"
 
     all_goals grind
 
@@ -173,7 +173,7 @@ aes_core.sub_bytes.sub_bytes_state st
       Vector.getElem_set_self, UInt16.toBitVec_not, UInt16.toBitVec_xor, UInt16.toBitVec_and,
       Nat.reduceEqDiff]
     simp only [<- var_24, <- var_2, <- var_4, <- var_6, <- var_8, <- var_10, <- var_12, <- var_14 ]
-    bv_check "./sat_proofs/sub_bytes_per_bit.lean-aes_core.sub_bytes.sub_bytes_correct-650-4.lrat"
+    bv_check "./sat_proofs/sub_bytes_correct.lrat"
   all_goals grind
 
 
@@ -198,23 +198,22 @@ aes_core.mix_columns.mix_columns_state_unrolled st
       | 0 | 1 | 2 | 3 | 4| 5 | 6 | 7 =>
         unfold aes_core.mix_columns.mix_columns_state_spec
         rename_auto_n 180
-        simp only [ne_eq, reduceCtorEq, not_false_eq_true, Vector.getElem_set_ne, Nat.succ_ne_self,
-          Vector.getElem_set_self, BitVec.natCast_eq_ofNat, Nat.reduceSubDiff, Nat.fold_succ,
-          Nat.fold_zero, Nat.zero_mul, Nat.sub_zero, Nat.one_mul, Nat.reduceMul,
-          Nat.sub_self]
+        simp only [ne_eq, Nat.reduceEqDiff, not_false_eq_true, Vector.getElem_set_ne,
+          Nat.succ_ne_self, reduceCtorEq, Vector.getElem_set_self, BitVec.natCast_eq_ofNat,
+          BitVec.ofNat_eq_ofNat, Nat.fold_succ, Nat.fold_zero, Nat.zero_mul, BitVec.zero_add,
+          Nat.one_mul, BitVec.reduceAdd, Nat.reduceMul]
         simp only [set_elem_bv, get_elem_bv, zero_array]
-        simp only [ne_eq, Nat.reduceEqDiff, not_false_eq_true, Vector.getElem_set_ne, reduceCtorEq,
-          Vector.getElem_set_self, Nat.sub_zero, Nat.reduceAdd, BitVec.zero_eq,
-          UInt16.ofBitVec_ofNat, Vector.getElem_replicate, UInt16.toBitVec_ofNat, BitVec.reduceBEq,
-          Bool.false_eq_true, ↓reduceIte, BitVec.shiftLeft_eq', BitVec.toNat_ofNat, Nat.reducePow,
-          Nat.zero_mod, BitVec.shiftLeft_zero, BitVec.reduceNot, BitVec.zero_and,
-          BitVec.ushiftRight_eq', BitVec.ushiftRight_zero, BitVec.zero_or, BEq.rfl, Nat.one_mod,
-          Nat.reduceMod, Vector.getElem_mk, List.getElem_toArray, List.getElem_cons_zero,
-          UInt16.toBitVec_ofBitVec, BitVec.reduceHShiftLeft, UInt16.ofBitVec_or,
-          UInt16.ofBitVec_and, Nat.reduceLT, UInt16.ofBitVec_shiftLeft, UInt16.ofNat_one,
-          List.getElem_cons_succ, UInt16.toBitVec_or, UInt16.toBitVec_and,
-          UInt16.toBitVec_shiftLeft, BitVec.ofNat_eq_ofNat, BitVec.reduceMod, UInt16.reduceOfNat,
-          Nat.lt_add_one]
+        simp only [Nat.sub_zero, Nat.reduceAdd, BitVec.zero_eq, UInt16.ofBitVec_ofNat,
+          Vector.getElem_replicate, UInt16.toBitVec_ofNat, BitVec.truncate_eq_setWidth,
+          Nat.reduceLeDiff, Nat.reducePow, Nat.zero_lt_succ, BitVec.setWidth_ofNat_of_le_of_lt,
+          BitVec.shiftLeft_eq', BitVec.toNat_ofNat, Nat.zero_mod, BitVec.shiftLeft_zero,
+          BitVec.reduceNot, BitVec.zero_and, BitVec.ushiftRight_eq', BitVec.ushiftRight_zero,
+          BitVec.zero_or, Nat.reduceLT, Nat.one_mod, Nat.reduceMod, Vector.getElem_mk,
+          List.getElem_toArray, List.getElem_cons_zero, UInt16.toBitVec_ofBitVec,
+          BitVec.reduceHShiftLeft, UInt16.ofBitVec_or, UInt16.ofBitVec_and,
+          UInt16.ofBitVec_shiftLeft, UInt16.ofNat_one, List.getElem_cons_succ, UInt16.toBitVec_or,
+          UInt16.toBitVec_and, UInt16.toBitVec_shiftLeft, BitVec.ofNat_eq_ofNat, BitVec.reduceMod,
+          UInt16.reduceOfNat, Nat.lt_add_one]
         simp only [GF8.add, GF8.mul_02_eq_xtime_bv, GF8.mul_03_eq_mul3_bv, GF8.mul3_bv, GF8.xtime_bv]
         rw_vars 81 to 148
         simp only [<- var_81, <- var_89, <- var_97, <- var_105, <- var_113, <- var_121, <- var_129, <- var_137 ]
