proofs/shift_rows_state.lean
@@ -5,6 +5,7 @@ import Hax
 import Std.Tactic.Do
 import Std.Do.Triple
 import Std.Tactic.Do.Syntax
+import Utilities
 
 open Std.Do
 open Std.Tactic
@@ -15,16 +16,22 @@ set_option linter.unusedVariables false
 
 namespace aes_core.shift_row_state
 
+def fst_row := [0, 4, 8, 12]
+def snd_row := [1, 5, 9, 13]
+def thrd_row := [2, 6, 10, 14]
+def frth_row := [3, 7, 11, 15]
 
+--For each map of bits we are moving the lements a number of positions depending
+-- on the row they are in the matrix.
 def shift_row_u16_spec (input : u16) : u16 :=
   let input_bitvec := input.toBitVec
   (16 : Nat).fold (init := 0) fun i _ res =>
     let bt := ((input_bitvec >>> i) &&& 1)
     res ||| UInt16.ofBitVec
-      (if i ∈ [0, 4, 8, 12] then bt <<< i else
-      if i ∈ [1, 5, 9, 13] then bt <<< ((i + 12) % 16) else
-      if i ∈ [2, 6, 10, 14] then bt <<< ((i + 8) % 16) else
-      --if i ∈ [3, 7, 11, 15] then
+      (if i ∈ fst_row then bt <<< i else
+      if i ∈ snd_row then bt <<< ((i + 12) % 16) else
+      if i ∈ thrd_row then bt <<< ((i + 8) % 16) else
+      --if i ∈ frth_row then
       bt <<< ((i + 4) % 16))
 
 @[spec]
@@ -37,6 +44,7 @@ def shift_row_u16 (input : u16) : RustM u16 := do
       |||? (← ((← (input &&&? (32768 : u16))) >>>? (12 : i32)))))
     |||? (← ((← (input &&&? (2184 : u16))) <<<? (4 : i32))))
 
+-- Apply the shift_rows to each of the map of bits.
 def shift_rows_stat_spec (st : (RustArray u16 8)) : Vector u16 8 :=
   st.toVec.map (shift_row_u16_spec)
 
@@ -98,7 +106,7 @@ shift_row_u16 input
     hax_mvcgen
     <;> simp at *
     .
-      unfold shift_row_u16_spec
+      unfold shift_row_u16_spec fst_row snd_row thrd_row
       simp
       rename_i h1 h2 h3 h4 h5 h6 h7 h8 h9 h10 h11 h12 h13
       unfold UInt16.lor
@@ -107,7 +115,5 @@ shift_row_u16 input
       clear h8 h9 h10 h11 h12 h13
       clear h1 h2 h3 h4 h5 h6 h7
       bv_decide
-
-
 
 end aes_core.shift_row_state
