proofs/transpose_u8x16.lean
@@ -2,6 +2,7 @@ import Hax
 import Std.Tactic.Do
 import Std.Do.Triple
 import Std.Tactic.Do.Syntax
+import Utilities
 
 open Std.Do
 open Std.Tactic
@@ -156,5 +157,37 @@ def transposeU8toU16 (input : RustArray u8 16) : RustArray u16 8 :=
   RustArray.ofVec <| Vector.ofFn fun (bt_num : Fin 8) =>
     (16 : Nat).fold (init := (0 : u16)) fun mtx_elem_num _ bt_plane =>
       UInt16.ofBitVec (bt_plane.toBitVec ||| (((input.toVec[mtx_elem_num].toBitVec >>> bt_num.val) &&& 1).setWidth 16 <<< mtx_elem_num))
+
+#eval transposeU8toU16 (RustArray.ofVec #v[(0x1 : u8), 2, 3, 0, 0, 0 , 0, 0, 0, 0, 0, 0, 0 , 0, 1, 1])
+
+--Theorem to ensure that we can obtain the same elements from the input
+set_option maxHeartbeats 10000000
+theorem transpose_correct (input : (RustArray u8 16)) (i : Nat) (hi : i < 16) :
+  get_elem_bv (transposeU8toU16 input).toVec (BitVec.ofFin ⟨i, hi⟩) = input.toVec[i].toBitVec := by
+  simp
+  match i with
+  | n + 16 => grind
+  | 0 | 1 | 2 | 3 | 4 | 5 | 6 | 7 | 8 | 9 | 10 | 11 | 12 | 13 | 14 | 15 =>
+
+    simp only [get_elem_bv, transposeU8toU16]
+    simp
+    generalize h0 : @getElem (Vector u8 16) Nat u8 (fun x i => i < 16) Vector.instGetElemNatLt input.toVec 0 _ = var_0
+    generalize h1 : @getElem (Vector u8 16) Nat u8 (fun x i => i < 16) Vector.instGetElemNatLt input.toVec 1 _ = var_1
+    generalize h2 : @getElem (Vector u8 16) Nat u8 (fun x i => i < 16) Vector.instGetElemNatLt input.toVec 2 _ = var_2
+    generalize h3 : @getElem (Vector u8 16) Nat u8 (fun x i => i < 16) Vector.instGetElemNatLt input.toVec 3 _ = var_3
+    generalize h4 : @getElem (Vector u8 16) Nat u8 (fun x i => i < 16) Vector.instGetElemNatLt input.toVec 4 _ = var_4
+    generalize h5 : @getElem (Vector u8 16) Nat u8 (fun x i => i < 16) Vector.instGetElemNatLt input.toVec 5 _ = var_5
+    generalize h6 : @getElem (Vector u8 16) Nat u8 (fun x i => i < 16) Vector.instGetElemNatLt input.toVec 6 _ = var_6
+    generalize h7 : @getElem (Vector u8 16) Nat u8 (fun x i => i < 16) Vector.instGetElemNatLt input.toVec 7 _ = var_7
+    generalize h8 : @getElem (Vector u8 16) Nat u8 (fun x i => i < 16) Vector.instGetElemNatLt input.toVec 8 _ = var_8
+    generalize h9 : @getElem (Vector u8 16) Nat u8 (fun x i => i < 16) Vector.instGetElemNatLt input.toVec 9 _ = var_9
+    generalize h10 : @getElem (Vector u8 16) Nat u8 (fun x i => i < 16) Vector.instGetElemNatLt input.toVec 10 _ = var_10
+    generalize h11 : @getElem (Vector u8 16) Nat u8 (fun x i => i < 16) Vector.instGetElemNatLt input.toVec 11 _ = var_11
+    generalize h12 : @getElem (Vector u8 16) Nat u8 (fun x i => i < 16) Vector.instGetElemNatLt input.toVec 12 _ = var_12
+    generalize h13 : @getElem (Vector u8 16) Nat u8 (fun x i => i < 16) Vector.instGetElemNatLt input.toVec 13 _ = var_13
+    generalize h14 : @getElem (Vector u8 16) Nat u8 (fun x i => i < 16) Vector.instGetElemNatLt input.toVec 14 _ = var_14
+    generalize h15 : @getElem (Vector u8 16) Nat u8 (fun x i => i < 16) Vector.instGetElemNatLt input.toVec 15 _ = var_15
+
+    bv_decide
 
 end aes_core.transpose_u8x16
